perm.v
@@ -1,0 +1,54 @@
+From iris.program_logic Require Import thread_local.
+From lrust Require Export type.
+
+Delimit Scope perm_scope with P.
+Bind Scope perm_scope with perm.
+
+Module Perm.
+
+Section perm.
+
+  Context `{lifetimeG Σ}.
+
+  (* TODO : define valuable expressions ν in order to define ν ◁ τ. *)
+
+  Definition extract (κ : lifetime) (ρ : perm) : perm :=
+    λ tid, (κ ∋ ρ tid)%I.
+
+  Definition tok (κ : lifetime) (q : Qp) : perm :=
+    λ _, ([κ]{q} ★ lft κ)%I.
+
+  Definition incl (κ κ' : lifetime) : perm :=
+    λ _, (κ ⊑ κ')%I.
+
+  Definition exist {A : Type} (P : A -> perm) : @perm Σ :=
+    λ tid, (∃ x, P x tid)%I.
+
+  Definition sep (ρ1 ρ2 : perm) : @perm Σ :=
+    λ tid, (ρ1 tid ★ ρ2 tid)%I.
+
+  Definition top : @perm Σ :=
+    λ _, True%I.
+
+End perm.
+
+End Perm.
+
+Import Perm.
+
+Notation "κ ∋ ρ" := (extract κ ρ)
+  (at level 75, right associativity) : perm_scope.
+
+Notation "[ κ ]{ q }" := (tok κ q) (format "[ κ ]{ q }") : perm_scope.
+
+Infix "⊑" := incl (at level 70) : perm_scope.
+
+Notation "∃ x .. y , P" :=
+  (exist (λ x, .. (exist (λ y, P)) ..)) : perm_scope.
+
+Infix "★" := sep (at level 80, right associativity) : perm_scope.
+
+Notation "⊤" := top : perm_scope.
+
+Definition perm_incl {Σ} (ρ1 ρ2 : @perm Σ) :=
+  ∀ tid, ρ1 tid ⊢ ρ2 tid.
