type_incl.v
@@ -1,0 +1,119 @@
+From iris.algebra Require Import upred_big_op.
+From iris.program_logic Require Import thread_local.
+From lrust Require Export type perm.
+
+Import Types.
+
+Section ty_incl.
+
+  Context `{heapG Σ, lifetimeG Σ, thread_localG Σ}.
+
+  Definition ty_incl (ρ : perm) (ty1 ty2 : type) :=
+    ∀ tid,
+      ρ tid ⊢
+      (□ ∀ tid vl, ty1.(ty_own) tid vl → ty2.(ty_own) tid vl) ∧
+      (□ ∀ κ tid E l, ty1.(ty_shr) κ tid E l →
+                      ty2.(ty_shr) κ tid E l
+       (* [ty_incl] needs to prove something about the length of the
+          object when it is shared. We place this property under the
+          hypothesis that [ty2.(ty_shr)] holds, so that the [!]  type
+          is still included in any other. *)
+                    ★ ty1.(ty_size) = ty2.(ty_size)).
+
+  Lemma ty_incl_refl ρ ty : ty_incl ρ ty ty.
+  Proof. iIntros (tid0) "_". iSplit; iIntros "!#"; eauto. Qed.
+
+  Lemma ty_incl_trans ρ ty1 ty2 ty3 :
+    ty_incl ρ ty1 ty2 → ty_incl ρ ty2 ty3 → ty_incl ρ ty1 ty3.
+  Proof.
+    iIntros (H12 H23 tid0) "H".
+    iDestruct (H12 with "H") as "[#H12 #H12']".
+    iDestruct (H23 with "H") as "[#H23 #H23']".
+    iSplit; iIntros "{H}!#*H1".
+    - by iApply "H23"; iApply "H12".
+    - iDestruct ("H12'" $! _ _ _ _ with "H1") as "[H2 %]".
+      iDestruct ("H23'" $! _ _ _ _ with "H2") as "[$ %]".
+      iPureIntro. congruence.
+  Qed.
+
+  Lemma ty_weaken ρ θ ty1 ty2 :
+    perm_incl ρ θ → ty_incl θ ty1 ty2 → ty_incl ρ ty1 ty2.
+  Proof. iIntros (Hρθ Hθ tid) "H". iApply Hθ. by iApply Hρθ. Qed.
+
+  Lemma ty_incl_bot ρ ty : ty_incl ρ ! ty.
+  Proof. iIntros (tid0) "_". iSplit; iIntros "!#*/=[]". Qed.
+
+  Lemma ty_incl_own ρ ty1 ty2 q :
+    ty_incl ρ ty1 ty2 → ty_incl ρ (own q ty1) (own q ty2).
+  Proof.
+    iIntros (Hincl tid0) "H/=". iDestruct (Hincl with "H") as "[#Howni #Hshri]".
+    iClear "H". iSplit; iIntros "!#*H".
+    - iDestruct "H" as (l) "(%&H†&Hmt)". subst. iExists _. iSplit. done.
+      iDestruct "Hmt" as (vl') "[Hmt Hown]". iNext.
+      iDestruct (ty_size_eq with "Hown") as %<-.
+      iDestruct ("Howni" $! _ _ with "Hown") as "Hown".
+      iDestruct (ty_size_eq with "Hown") as %<-. iFrame.
+      iExists _. by iFrame.
+    - iDestruct "H" as (l') "[Hfb #Hvs]". iSplit; last done. iExists l'. iFrame.
+      iIntros (q') "!#Hκ".
+      iVs ("Hvs" $! _ with "Hκ") as "Hvs'". iIntros "!==>!>".
+      iVs "Hvs'" as "[Hshr $]". iVsIntro.
+      by iDestruct ("Hshri" $! _ _ _ _ with "Hshr") as "[$ _]".
+  Qed.
+
+  Lemma lft_incl_ty_incl_uniq_borrow ρ ty κ1 κ2 :
+    perm_incl ρ (κ1 ⊑ κ2) → ty_incl ρ (&uniq{κ2}ty) (&uniq{κ1}ty).
+  Proof.
+    iIntros (Hκκ' tid0) "H". iDestruct (Hκκ' with "H") as "#Hκκ'". iClear "H".
+    iSplit; iIntros "!#*H".
+    - iDestruct "H" as (l) "[% Hown]". subst. iExists _. iSplit. done.
+      by iApply (lft_borrow_incl with "Hκκ'").
+    - admit. (* TODO : fix the definition before *)
+  Admitted.
+
+  Lemma lft_incl_ty_incl_shared_borrow ρ ty κ1 κ2 :
+    perm_incl ρ (κ1 ⊑ κ2) → ty_incl ρ (&shr{κ2}ty) (&shr{κ1}ty).
+  Proof.
+    iIntros (Hκκ' tid0) "H". iDestruct (Hκκ' with "H") as "#Hκκ'". iClear "H".
+    iSplit; iIntros "!#*H".
+    - iDestruct "H" as (l) "[% Hown]". subst. iExists _. iSplit. done.
+      by iApply (ty.(ty_shr_mono) with "Hκκ'").
+    - iDestruct "H" as (vl) "#[Hfrac Hty]". iSplit; last done.
+      iExists vl. iFrame "#". iNext.
+      iDestruct "Hty" as (l0) "[% Hty]". subst. iExists _. iSplit. done.
+      by iApply (ty_shr_mono with "Hκκ' Hty").
+  Qed.
+
+  Lemma ty_incl_prod ρ tyl1 tyl2 :
+    Forall2 (ty_incl ρ) tyl1 tyl2 → ty_incl ρ (product tyl1) (product tyl2).
+  Proof.
+    rewrite {2}/ty_incl /product /=. iIntros (HFA tid0) "Hρ". iSplit.
+    - assert (Himpl : ρ tid0 ⊢
+         □ (∀ tid vll, length tyl1 = length vll →
+               ([★ list] tyvl ∈ combine tyl1 vll, ty_own (tyvl.1) tid (tyvl.2))
+             → ([★ list] tyvl ∈ combine tyl2 vll, ty_own (tyvl.1) tid (tyvl.2)))).
+      { induction HFA as [|ty1 ty2 tyl1 tyl2 Hincl HFA IH].
+        - iIntros "_!#* _ _". by rewrite big_sepL_nil.
+        - iIntros "Hρ". iDestruct (IH with "Hρ") as "#Hqimpl".
+          iDestruct (Hincl with "Hρ") as "[#Hhimpl _]". iIntros "!#*%".
+          destruct vll as [|vlh vllq]. discriminate. rewrite !big_sepL_cons.
+          iIntros "[Hh Hq]". iSplitL "Hh". by iApply "Hhimpl".
+          iApply ("Hqimpl" with "[] Hq"). iPureIntro. simpl in *. congruence. }
+      iDestruct (Himpl with "Hρ") as "#Himpl". iIntros "{Hρ}!#*H".
+      iDestruct "H" as (vll) "(%&%&H)". iExists _. iSplit. done. iSplit.
+      by rewrite -(Forall2_length _ _ _ HFA). by iApply ("Himpl" with "[] H").
+    - iRevert "Hρ". generalize O.
+      change (ndot (A:=nat)) with (λ N i, N .@ (0+i)%nat). generalize O.
+      induction HFA as [|ty1 ty2 tyl1 tyl2 Hincl HFA IH].
+      + iIntros (i offs) "_!#* _". rewrite big_sepL_nil. eauto.
+      + iIntros (i offs) "Hρ". iDestruct (IH with "[] Hρ") as "#Hqimpl". done.
+        iDestruct (Hincl with "Hρ") as "[_ #Hhimpl]". iIntros "!#*".
+        rewrite !big_sepL_cons. iIntros "[Hh Hq]".
+        setoid_rewrite <-Nat.add_succ_comm.
+        iDestruct ("Hhimpl" $! _ _ _ _ with "Hh") as "[$ %]".
+        replace ty2.(ty_size) with ty1.(ty_size) by done.
+        iDestruct ("Hqimpl" $! _ _ _ _ with "Hq") as "[$ %]".
+        iIntros "!%/=". congruence.
+  Qed.
+
+End ty_incl.
